@prefix rdfs: <http://www.w3.org/2000/01/rdf-schema#>.
@prefix rdf: <http://www.w3.org/1999/02/22-rdf-syntax-ns#>.
@prefix xsd: <http://www.w3.org/2001/XMLSchema#>.
@prefix qr: <http://purl.org/eis/vocab/qr#>.
@prefix owl: <http://www.w3.org/2002/07/owl#>.
@prefix daq: <http://purl.org/eis/vocab/daq#>.


# Classes
qr:QualityReport a rdfs:Class ;
	rdfs:comment "Represents a report on the problems detected during the assessment of quality on a dataset." ;
	rdfs:label "Quality Report" .
	
qr:QualityProblem a rdfs:Class ;
	rdfs:comment "Represents a quality problem detected during the assessment of quality metrics on triples." ;
	rdfs:label "Quality Problem" .
	
qr:CleaningRecommendation a rdfs:Class ;
	rdfs:comment "Represents recommendation for how to solve the corresponding quality problem." ;
	rdfs:label "Cleaning Suggestion" .
	
qr:MalformedDatatypeLiteralsProblem a rdfs:Class ;
	rdfs:subClassOf qr:QualityProblem ;
	rdfs:comment "Represents a kind of quality problems in which literal value is not consistent with defined data type" ;
	qr:problemDescription "Literal value is not consistent with the defined data type.";
	rdfs:label "Malformed Datatype literals Problem" . 
	
qr:MalformedDatatypeLiteralsRecommendation a rdfs:Class ;
	rdfs:subClassOf qr:CleaningRecommendation ;
	rdfs:comment "Represents recommendation of how to solve the corresponding quality problem";
	qr:recommedation "Parse or convert literal into the value space of the data type." ;
	rdfs:label "Malformed Datatype literals Recommendation" .

qr:IncompatibleDatatypeRangeProblem a rdfs:Class ;
	rdfs:subClassOf qr:QualityProblem ;
	rdfs:comment "Represents a kind of quality problems in which literal value is not consistent with data type defined by property range" ; 
	qr:problemDescription "Literal value is not consistent with data type defined by property range" ;
	rdfs:label "Incompatible Datatype Range Problem " . 
	
qr:IncompatibleDatatypeRangeRecommendation a rdfs:Class ;
	rdfs:subClassOf qr:CleaningRecommendation ;
	rdfs:comment "Represents recommendation of how to solve the corresponding quality problem";
	qr:recommedation "Parse or convert the literal value into the value space of the range datatype" ;
	rdfs:label "Incompatible Datatype Range Recommendation " .

qr:HomogeneousDatatypesProblem a rdfs:Class ;
	rdfs:subClassOf qr:QualityProblem ;
	qr:problemDescription "Data type of literals corresponding to the same property is not homogeneous" ;
	rdfs:comment "Represents a kind of quality problems in which data type are not homogeneous" ;
	rdfs:label "Homogeneous Datatype Problem " . 
	
qr:HomogeneousDatatypesRecommendation a rdfs:Class ;
	rdfs:subClassOf qr:CleaningRecommendation ;
	rdfs:comment "Represents recommendation of how to solve the corresponding quality problem";
	qr:recommedation "Parse or convert literal values to unique data type" ;
	rdfs:label "Homogeneous Datatype Recommendation " . 

qr:MisplacedClassesOrPropertiesProblem a rdfs:Class ;
	rdfs:subClassOf qr:QualityProblem ;
	rdfs:comment "Represents a kind of quality problems in which classes or properties are not places properly." ;
	rdfs:label "Misplaced classes or properties Problem " . 

qr:MisuseOwlDatatypeOrObjectPropertiesProblem a rdfs:Class ;
	rdfs:subClassOf qr:QualityProblem ;
	rdfs:comment "Represents a kind of quality problems in which owl classes or owl properties are not used properly." ;
	rdfs:label "Misuse Owl Datatype Or Object Properties Problem" .

qr:UndefinedClassesProblem a rdfs:Class ;
	rdfs:subClassOf qr:QualityProblem ;
	qr:problemDescription "Class is not defined." ;
	rdfs:comment "Represents a kind of quality problems in which classes are not defined" ;
	rdfs:label "Undefined Classes Problem" .
	
qr:UndefinedClassesRecommendation a rdfs:Class ;
	rdfs:subClassOf qr:CleaningRecommendation;	
	rdfs:comment "Represents recommendation of how to solve the corresponding quality problem";
	qr:recommedation "Please define the class" ;
	rdfs:label "Undefined Classes Recommendation" .
	
qr:UndefinedPropertiesProblem a rdfs:Class ;
	rdfs:subClassOf qr:QualityProblem ;
	qr:problemDescription "Property is not defined." ;
	rdfs:comment "Represents a kind of quality problems in which classes or properties are not defined" ;
	rdfs:label "Undefined Properties Problem".
	
qr:UndefinedPropertiesRecommendation a rdfs:Class ;
	rdfs:subClassOf qr:CleaningRecommendation;
	rdfs:comment "Represents recommendation of how to solve the corresponding quality problem";
	qr:recommedation "Please define the property." ;
	rdfs:label "Undefined Properties Recommendation".
	
qr:WhitespaceInAnnotationProblem a rdfs:Class ;
	rdfs:subClassOf qr:QualityProblem ;
	qr:problemDescription "Literal value contains white spaces";
	rdfs:comment "Represents a kind of quality problems in which object in annotation property contains white spaces." ;
	rdfs:label "Whitespace in Annotation Problem".
	
qr:WhitespaceInAnnotationRecommendation a rdfs:Class ;
	rdfs:subClassOf qr:CleaningRecommendation;
	rdfs:comment "Represents recommendation of how to solve the corresponding quality problem";
	qr:recommedation "Remove white spaces from the literal value" ;
	rdfs:label "Whitespace in Annotation Recommendation".
	
qr:EmptyAnnotationValueProblem a rdfs:Class ;
	rdfs:subClassOf qr:QualityProblem ;
	rdfs:comment "Represents a kind of quality problems in which literal value in annotation property is empty." ;
	rdfs:label "Empty Annotation Value Problem".
	
qr:EmptyAnnotationValueRecommendation a rdfs:Class ;
	rdfs:subClassOf qr:CleaningRecommendation;
	rdfs:comment "Represents recommendation of how to solve the corresponding quality problem";
	qr:recommedation "Remove the triple or add literal value" ;
	rdfs:label "Empty Annotation Value Recommendation".
	
qr:LabelsUsingCapitalsProblem a rdfs:Class ;
	rdfs:subClassOf qr:QualityProblem ;
	rdfs:comment "Represents a kind of quality problems in which object value in label property uses a bad style of capitalization." ;
	rdfs:label "Labels Using Capitals Problem".
	
qr:LabelsUsingCapitalsRecommendation a rdfs:Class ;
	rdfs:subClassOf qr:CleaningRecommendation;
	rdfs:comment "Represents recommendation of how to solve the corresponding quality problem";
	qr:recommedation "Change the capitalization of the literal";
	rdfs:label "Labels Using Capitals Recommendation".
	
qr:BlankNodeUsageProblem a rdfs:Class ;
	rdfs:subClassOf qr:QualityProblem ;
	rdfs:comment "Represents a kind of quality problems in which blank nodes are used in subject or object position." ;
	rdfs:label "Blank Node Usage Problem".
	
qr:BlankNodeUsageRecommendation a rdfs:Class ;
	rdfs:subClassOf qr:CleaningRecommendation;
	rdfs:comment "Represents recommendation of how to solve the corresponding quality problem";
	qr:recommedation "Assign an URI to the node";
	rdfs:label "Blank Node Usage Recommendation".

qr:RDFAccessibilityProblem a rdfs:Class ;
	rdfs:subClassOf qr:QualityProblem ;
	rdfs:comment "Represents a kind of quality problems when RDF can not be accessed." ;
	rdfs:label "RDF Accessibility Problem".
	
qr:RDFAccessibilityRecommendation a rdfs:Class ;
	rdfs:subClassOf qr:CleaningRecommendation;
	rdfs:comment "Represents recommendation of how to solve the corresponding quality problem";
	qr:recommedation "Check the path to RDF dump or remove the triple";
	rdfs:label "RDF Accessibility Recommendation".
	
qr:SPARQLAccessibilityProblem a rdfs:Class ;
	rdfs:subClassOf qr:QualityProblem ;
	rdfs:comment "Represents a kind of quality problems when SPARQL Endpoint can not be accessed." ;
	rdfs:label "SPARQL Accessibility Problem".
	
qr:SPARQLAccessibilityRecommendation a rdfs:Class ;
	rdfs:subClassOf qr:CleaningRecommendation;
	rdfs:comment "Represents recommendation of how to solve the corresponding quality problem";
	qr:recommedation "Check the SPARQL Endpoint  URI or remove the triple";
	rdfs:label "SPARQL Accessibility Recommendation".
		
qr:DefinedOntologyAuthorProblem a rdfs:Class ;
	rdfs:subClassOf qr:QualityProblem ;
	rdfs:comment "Identifies when an ontology author is not defined." ;
	rdfs:label "Defined Ontology Author Problem".	
	
		
qr:DefinedOntologyAuthorRecommendation a rdfs:Class ;
	rdfs:subClassOf qr:CleaningRecommendation;
	rdfs:comment "Represents recommendation of how to solve the corresponding quality problem";
	qr:recommedation "Define the ontology author";
	rdfs:label "Defined Ontology Author Recommendation".	
	
	
# Properties
qr:computedOn a rdf:Property ;
	rdfs:comment "Represents the dataset URI on which quality metrics where computed" ;
	rdfs:domain qr:QualityReport ;
	rdfs:label "computedOn" ;
	rdfs:range rdfs:Resource .
	
qr:hasProblem a rdf:Property ;
	rdfs:comment "Identifies problem instances in the report";
	rdfs:domain qr:QualityReport ;
	rdfs:label "has Problem" ;
	rdfs:range qr:QualityProblem .

qr:isDescribedBy a rdf:Property;
	rdfs:comment "Represent the URI of the metric which instantiated this problem";
	rdfs:domain qr:QualityProblem;
	rdfs:label "isDescribedBy";
	rdfs:range daq:Metric.

qr:problematicThing a rdf:Property;
	rdfs:comment "Represent the actual problematic instance from the dataset. This could be a list of resources (rdf:Seq) or a list of reified statements.";
	rdfs:domain qr:QualityProblem;
	rdfs:label "affects";
	rdfs:range rdfs:Resource.
	
qr:aplicableTo a rdf:Property ;
	rdfs:comment "Represents the relation between cleaning recommendation and quality problem." ;
	rdfs:domain qr:CleaningRecommendation ;
	rdfs:label "aplicableTo" ;
	rdfs:range qr:QualityProblem.
	
qr:problemDescription
		a	rdf:Property, owl:DatatypeProperty ;
		rdfs:label	"problemDescription" ;
		rdfs:comment	"Contains brief summary of the quality problem that is presented to the user." ;
		rdfs:domain	qr:QualityProblem;
		rdfs:range	 xsd:string.
		
qr:recommedation
		a	rdf:Property, owl:DatatypeProperty ;
		rdfs:label	"recommendation" ;
		rdfs:comment	"Contains recommendation of how to solve the corresponding quality problem." ;
		rdfs:domain	qr:CleaningRecommendation;
		rdfs:range	 xsd:string.
		