@prefix daq:     <http://purl.org/eis/vocab/daq#> .
@prefix dqm:     <http://www.diachron-fp7.eu/dqm#> .
@prefix owl:	 <http://www.w3.org/2002/07/owl#> .
@prefix rdf:     <http://www.w3.org/1999/02/22-rdf-syntax-ns#> .
@prefix rdfg:	 <http://www.w3.org/2004/03/trix/rdfg-1> .
@prefix rdfs:    <http://www.w3.org/2000/01/rdf-schema#> .
@prefix xsd:     <http://www.w3.org/2001/XMLSchema#> .


	#Category Classes
	dqm:Accessibility
		a	rdfs:Class ;
		rdfs:subClassOf	daq:Category ;
		rdfs:comment	"Encompasses dimensions related to the ability to access to and retrieve the dataset required for a particular use case" ;
		rdfs:label	"Accessibility" .
		
	dqm:Intrinsic
		a	rdfs:Class ;
		rdfs:subClassOf	daq:Category ;
		rdfs:comment	"Refers to dimensions that are independent of the user's context and that measure the correctness, succinctness and consistency of the dataset" ;
		rdfs:label	"Intrinsic" .
		
	dqm:Trust
		a	rdfs:Class ;
		rdfs:subClassOf	daq:Category ;
		rdfs:comment	"Dimensions belonging to this group focus on the perceived trustworthiness of the dataset and its sources" ;
		rdfs:label	"Trust" .
		
	dqm:Dynamicity
		a	rdfs:Class ;
		rdfs:subClassOf	daq:Category ;
		rdfs:comment	"Dimensions in this category provide information about how current is the data (i.e. its freshness over time) and how frequently it changes" ;
		rdfs:label	"Dynamicity" .
	
	dqm:Contextual
		a	rdfs:Class ;
		rdfs:subClassOf	daq:Category ;
		rdfs:comment	"Comprises dimensions that highly depend on the context of the task to be performed" ;
		rdfs:label	"Contextual" .
		
	dqm:Representational
		a	rdfs:Class ;
		rdfs:subClassOf	daq:Category ;
		rdfs:comment	"Groups dimensions related to the design of the data, which provide information about how the chosen representation of the data affect its quality" ;
		rdfs:label	"Representational" .

	#Dimension Classes
	dqm:Availability
		a	rdfs:Class ;
		rdfs:subClassOf	daq:Dimension ;
		rdfs:comment	"Metrics in this dimension measure the extent to which information (or some portion of it) is present, obtainable and ready for use" ;
		rdfs:label	"Availability" .
		
	dqm:Accuracy
		a	rdfs:Class ;
		rdfs:subClassOf	daq:Dimension ;
		rdfs:comment	"Extent to which data is correct. The degree to which the dataset correctly represents the real world and how much it is free of syntax errors. Classified in: Syntactic accuracy (the degree to which data values are close to their definition domain) and Semantic accuracy (the degree to which data values correctly represent the actual real world values)" ;
		rdfs:label	"Accuracy" .
			
	dqm:AmountOfData
		a	rdfs:Class ;
		rdfs:subClassOf	daq:Dimension ;
		rdfs:comment	"Refers to how appropriate the quantity and volume of data is for the task at hand. The amount of data should be enough to approximate the true scenario precisely" ;
		rdfs:label	"Amount of Data" .
	
	dqm:Conciseness
		a	rdfs:Class ;
		rdfs:subClassOf	daq:Dimension ;
		rdfs:comment	"Refers to the redundancy of entities, be it at the schema or the data level" ;
		rdfs:label	"Conciseness" .
		
	dqm:RepresentationalConciseness
		a	rdfs:Class ;
		rdfs:subClassOf	daq:Dimension ;
		rdfs:comment	"Measures the extent to which the representation of data is compact, clear and well formatted" ;
		rdfs:label	"RepresentationalConciseness" .
		
	dqm:Currency
		a	rdfs:Class ;
		rdfs:subClassOf	daq:Dimension ;
		rdfs:comment	"Provides a measure of the degree to which information is up to date and how promptly the data is updated" ;
		rdfs:label	"Currency" .

	#Metric Classes
	dqm:EndPointAvailabilityMetric
		a	rdfs:Class ;
		rdfs:subClassOf	daq:Metric ;
		rdfs:comment	"Checks whether the server (endpoint) is reachable and responds to a SPARQL query" ;
		rdfs:label	"EndPointAvailabilityMetric" .		

	dqm:RDFAvailabilityMetric
		a	rdfs:Class ;
		rdfs:subClassOf	daq:Metric ;
		rdfs:comment	"Upon request of an RDF dump, checks whether it is provided as result" ;
		rdfs:label	"RDFAvailabilityMetric" .	

	dqm:DereferenceabilityMetric
		a	rdfs:Class ;
		rdfs:subClassOf	daq:Metric ;
		rdfs:comment	"Determines whether requesting a resource, identified by a URI, results in an error code being returned (e.g. 4xx: client error or 5xx: server error), or in a broken link" ;
		rdfs:label	"DereferenceabilityMetric" .	

	dqm:UnstructuredMetric
		a	rdfs:Class ;
		rdfs:subClassOf	daq:Metric ;
		rdfs:comment	"Detects dead links or URIs without any supporting RDF metadata or no redirection using the status code 303" ;
		rdfs:label	"UnstructuredMetric" .			

	dqm:DereferenceabilityBackLinksMetric
		a	rdfs:Class ;
		rdfs:subClassOf	daq:Metric ;
		rdfs:comment	"Detects all local in-links or back-links (locally available triples with the resource URI appearing as object, in the dereferenced document returned for the resource)" ;
		rdfs:label	"DereferenceabilityBackLinksMetric" .	

	dqm:DereferenceabilityForwardLinksMetric
		a	rdfs:Class ;
		rdfs:subClassOf	daq:Metric ;
		rdfs:comment	"Detects all forward links (locally known triples where the local URI is mentioned in the subject)" ;
		rdfs:label	"DereferenceabilityForwardLinksMetric" .	

	dqm:MisreportedContentTypesMetric
		a	rdfs:Class ;
		rdfs:subClassOf	daq:Metric ;
		rdfs:comment	"Checks whether the content is suitable for consumption and if such content should be accessed" ;
		rdfs:label	"MisreportedContentTypesMetric" .	

	dqm:MalformedDatatypeLiteralsMetric
		a	rdfs:Class ;
		rdfs:subClassOf	daq:Metric ;
		rdfs:comment	"Detects ill-typed literals, which do not abide by the lexical syntax of their respective datatypes" ;
		rdfs:label	"MalformedDatatypeLiteralsMetric" .		

	dqm:AmountOfTriplesMetric
		a	rdfs:Class ;
		rdfs:subClassOf	daq:Metric ;
		rdfs:comment	"Counts the total number of triples present in the dataset" ;
		rdfs:label	"AmountOfTriplesMetric" .
		
	dqm:IntensionalConcisenessMetric
		a	rdfs:Class ;
		rdfs:subClassOf	daq:Metric ;
		rdfs:comment	"Provides a measure of the redundancy of the dataset at the schema level, computed as the ratio of the Number of Unique Attributes (Properties) to the Total Number of Attributes in the target schema" ;
		rdfs:label	"IntensionalConcisenessMetric" .
		
	dqm:ExtensionalConcisenessMetric
		a	rdfs:Class ;
		rdfs:subClassOf	daq:Metric ;
		rdfs:comment	"Provides a measure of the redundancy of the dataset at the data level, computed as the ratio of the Number of Unique Subjects to the Total Number of Subjects" ;
		rdfs:label	"ExtensionalConcisenessMetric" .
		
	dqm:DuplicateInstanceMetric
		a	rdfs:Class ;
		rdfs:subClassOf	daq:Metric ;
		rdfs:comment	"Provides a measure of the redundancy of entities at the data level (ratio of entities that violate the uniqueness rule)" ;
		rdfs:label	"DuplicateInstanceMetric" .
		
	dqm:ShortURIsMetric
		a	rdfs:Class ;
		rdfs:subClassOf	daq:Metric ;
		rdfs:comment	"Detects the use of short URIs (and the avoidance of query parameters), which suggests that information is compactly represented and favors readability" ;
		rdfs:label	"ShortURIsMetric" .
	
	dqm:CurrencyOfDocumentStatementsMetric
		a	rdfs:Class ;
		rdfs:subClassOf	daq:Metric ;
		rdfs:comment	"Compares the time when the data was observed with the time when the data (document as a whole and individual triples) were last modified, thereby providing a measure of how current the dataset is" ;
		rdfs:label	"CurrencyOfDocumentStatementsMetric" .
		
	dqm:TimeSinceModificationMetric
		a	rdfs:Class ;
		rdfs:subClassOf	daq:Metric ;
		rdfs:comment	"Provides a measure of the degree to which information is up to date, by comparing the current time with the time when the data was last modified" ;
		rdfs:label	"TimeSinceModificationMetric" .
	
	#Properties
	#Accessibility Dimensions Properties
	dqm:hasAvailabilityDimension
		a	rdfs:Property ;	
		rdfs:subPropertyOf	daq:hasDimension ;
		rdfs:comment	"Links Accessibility Category with Availability Dimension" ;
		rdfs:label	"hasAvailabilityDimension" ;
		rdfs:domain	dqm:Accessibility ;
		rdfs:range	dqm:Availability .
		
	#Availability Metric Properties
	dqm:hasEndPointAvailabilityMetric
		a	rdfs:Property ;
		rdfs:subPropertyOf	daq:hasMetric ;
		rdfs:comment	"Links Availability Dimension with Endpoint Availability Metric (Endpoint Availability Metric belongs to the Availability Dimension)" ;
		rdfs:label	"hasEndPointAvailabilityMetric" ;
		rdfs:domain	dqm:Availability ;
		rdfs:range	dqm:EndPointAvailabilityMetric .

	dqm:hasRDFAvailabilityMetric
		a	rdfs:Property ;
		rdfs:subPropertyOf	daq:hasMetric ;
		rdfs:comment	"Links Availability Dimension with RDF Availability Metric (RDF Availability Metric belongs to the Availability Dimension)" ;
		rdfs:label	"hasRDFAvailabilityMetric" ;
		rdfs:domain	dqm:Availability ;
		rdfs:range	dqm:RDFAvailabilityMetric .

	dqm:hasDereferenceabilityMetric
		a	rdfs:Property ;
		rdfs:subPropertyOf	daq:hasMetric ;
		rdfs:comment	"Links Availability Dimension with Dereferenceability Metric (Dereferenceability Metric belongs to the Availability Dimension)" ;
		rdfs:label	"hasDereferenceabilityMetric" ;
		rdfs:domain	dqm:Availability ;
		rdfs:range	dqm:DereferenceabilityMetric .

	dqm:hasUnstructuredMetric
		a	rdfs:Property ;
		rdfs:subPropertyOf	daq:hasMetric ;
		rdfs:comment	"Links Availability Dimension with Unstructured Data Metric (Unstructured Data Metric belongs to the Availability Dimension)" ;
		rdfs:label	"hasUnstructuredMetric" ;
		rdfs:domain	dqm:Availability ;
		rdfs:range	dqm:UnstructuredMetric .		

	dqm:hasDereferenceabilityBackLinksMetric
		a	rdfs:Property ;
		rdfs:subPropertyOf	daq:hasMetric ;
		rdfs:comment	"Links Availability Dimension with Dereferenceability of Back-links Metric (Dereferenceability of Back-links Metric belongs to the Availability Dimension)" ;
		rdfs:label	"hasDereferenceabilityBackLinksMetric" ;
		rdfs:domain	dqm:Availability ;
		rdfs:range	dqm:DereferenceabilityBackLinksMetric .

	dqm:hasDereferenceabilityForwardLinksMetric
		a	rdfs:Property ;
		rdfs:subPropertyOf	daq:hasMetric ;
		rdfs:comment	"Links Availability Dimension with Dereferenceability of Forward-links Metric (Dereferenceability of Forward-links Metric belongs to the Availability Dimension)" ;
		rdfs:label	"hasDereferenceabilityForwardLinksMetric" ;
		rdfs:domain	dqm:Availability ;
		rdfs:range	dqm:DereferenceabilityForwardLinksMetric .

	dqm:hasMisreportedContentTypesMetric
		a	rdfs:Property ;
		rdfs:subPropertyOf	daq:hasMetric ;
		rdfs:comment	"Links Availability Dimension with Misreported Content Types Metric (Misreported Content Types Metric belongs to the Availability Dimension)" ;
		rdfs:label	"hasMisreportedContentTypesMetric" ;
		rdfs:domain	dqm:Availability ;
		rdfs:range	dqm:MisreportedContentTypesMetric .		

	#Accuracy Dimensions Properties
	dqm:hasAccuracyDimension
		a	rdfs:Property ;
		rdfs:subPropertyOf	daq:hasDimension ;
		rdfs:comment	"Links Intrinsic Category with Accuracy Dimension" ;
		rdfs:label	"hasAccuracyDimension" ;
		rdfs:domain	dqm:Intrinsic ;
		rdfs:range	dqm:Accuracy .
		
	dqm:hasMalformedDatatypeLiteralsMetric
		a	rdfs:Property ;
		rdfs:subPropertyOf	daq:hasMetric ;
		rdfs:comment	"Links Accuracy Dimension with Malformed Data Type Literals Metric (Malformed Data Type Literals Metric belongs to the Accuracy Dimension)" ;
		rdfs:label	"hasMalformedDatatypeLiteralsMetric" ;
		rdfs:domain	dqm:Accuracy ;
		rdfs:range	dqm:MalformedDatatypeLiteralsMetric .

	#Contextual Dimensions Properties
	dqm:hasAmountOfDataDimension
		a	rdfs:Property ;
		rdfs:subPropertyOf	daq:hasDimension ;
		rdfs:comment	"Links Contextual Category with Amount of Data Dimension" ;
		rdfs:label	"hasAmountOfDataDimension" ;
		rdfs:domain	dqm:Contextual ;
		rdfs:range	dqm:AmountOfData .
		
	dqm:hasAmountOfTriplesMetric
		a	rdfs:Property ;
		rdfs:subPropertyOf	daq:hasMetric ;
		rdfs:comment	"Links Amount of Data Dimension with Amount of Triples Metric (Amount of Triples Metric belongs to the Amount of Data Dimension)" ;
		rdfs:label	"hasAmountOfTriplesMetric" ;
		rdfs:domain	dqm:AmountOfData ;
		rdfs:range	dqm:AmountOfTriplesMetric .	
		
	#Conciseness Dimensions Properties
	dqm:hasConcisenessDimension
		a rdfs:Property ;
		rdfs:subPropertyOf daq:hasDimension ;
		rdfs:comment "Links Intrinsic Category with Conciseness Dimension" ;
		rdfs:label "hasConcisenessDimension" ;
		rdfs:domain dqm:Intrinsic ;
		rdfs:range dqm:Conciseness .
	
	dqm:hasIntensionalConcisenessMetric
		a	rdfs:Property ;
		rdfs:subPropertyOf	daq:hasMetric ;
		rdfs:comment	"Links Conciseness Dimension with Intensional Conciseness Metric (Intensional Conciseness Metric belongs to the Conciseness Dimension)" ;
		rdfs:label	"hasIntensionalConcisenessMetric" ;
		rdfs:domain	dqm:Conciseness ;
		rdfs:range	dqm:IntensionalConcisenessMetric .	
		
	dqm:hasExtensionalConcisenessMetric
		a	rdfs:Property ;
		rdfs:subPropertyOf	daq:hasMetric ;
		rdfs:comment	"Links Conciseness Dimension with Extensional Conciseness Metric (Extensional Conciseness Metric belongs to the Conciseness Dimension)" ;
		rdfs:label	"hasExtensionalConcisenessMetric" ;
		rdfs:domain	dqm:Conciseness ;
		rdfs:range	dqm:ExtensionalConcisenessMetric .	
		
	dqm:hasDuplicateInstanceMetric
		a	rdfs:Property ;
		rdfs:subPropertyOf	daq:hasMetric ;
		rdfs:comment	"Links Conciseness Dimension with Duplicate Instance Metric (Duplicate Instance Metric belongs to the Conciseness Dimension)" ;
		rdfs:label	"hasDuplicateInstanceMetric" ;
		rdfs:domain	dqm:Conciseness ;
		rdfs:range	dqm:DuplicateInstanceMetric .
		
	#Representational Conciseness Dimension Properties
	dqm:hasRepresentationalConcisenessDimension
		a rdfs:Property ;
		rdfs:subPropertyOf daq:hasDimension ;
		rdfs:comment "Links Representational Category with Representational-Conciseness Dimension" ;
		rdfs:label "hasRepresentationalConcisenessDimension" ;
		rdfs:domain dqm:Representational ;
		rdfs:range dqm:RepresentationalConciseness .
		
	dqm:hasShortURIsMetric
		a	rdfs:Property ;
		rdfs:subPropertyOf	daq:hasMetric ;
		rdfs:comment	"Links Representational-Conciseness Dimension with Keeping URIs Short Metric (Keeping URIs Short Metric belongs to the Representational-Conciseness Dimension)" ;
		rdfs:label	"hasShortURIsMetric" ;
		rdfs:domain	dqm:RepresentationalConciseness ;
		rdfs:range	dqm:ShortURIsMetric .
		
	#Currency Dimension Properties
	dqm:hasCurrencyDimension
		a rdfs:Property ;
		rdfs:subPropertyOf daq:hasDimension ;
		rdfs:comment "Links the Dynamicity Category with the Currency Dimension" ;
		rdfs:label "hasCurrencyDimension" ;
		rdfs:domain dqm:Dynamicity ;
		rdfs:range dqm:Currency .

	dqm:hasCurrencyOfDocumentStatementsMetric
		a	rdfs:Property ;
		rdfs:subPropertyOf	daq:hasMetric ;
		rdfs:comment	"Links the Currency Dimension with the Currency of Document/Statements Metric (Currency of Document/Statements Metric belongs to the Currency Dimension)" ;
		rdfs:label	"hasCurrencyOfDocumentStatementsMetric" ;
		rdfs:domain	dqm:Currency ;
		rdfs:range	dqm:CurrencyOfDocumentStatementsMetric .

	dqm:hasTimeSinceModificationMetric
		a	rdfs:Property ;
		rdfs:subPropertyOf	daq:hasMetric ;
		rdfs:comment	"Links the Currency Dimension with the Time Since Modification Metric (Time Since Modification Metric belongs to the Currency Dimension)" ;
		rdfs:label	"hasTimeSinceModificationMetric" ;
		rdfs:domain	dqm:Currency ;
		rdfs:range	dqm:TimeSinceModificationMetric .